Valaig/Data.lean
@@ -4,3 +4,4 @@ public import Valaig.Data.AbsMap
 public import Valaig.Data.DetIter
 public import Valaig.Data.Pool
 public import Valaig.Data.Nullable
+public import Valaig.Data.VarCache
