Valaig/Data/VarCache.lean
@@ -1,0 +1,334 @@
+module
+
+public import Valaig.Refs
+import Valaig.ForLean.Array
+public import Valaig.Data.Nullable
+
+public section
+namespace Valaig.Data
+
+/--
+  An automatically growable cache between contiguous variables and an arbitrary other type.
+-/
+structure VarCache (α : Type) where
+  ofArray ::
+    cache : Array α
+deriving DecidableEq, Inhabited, Repr
+
+namespace VarCache
+variable {α : Type} {cache : VarCache α} {var : Var}
+
+@[inline, local simp, local grind]
+def size (cache : VarCache α) : Nat :=
+  cache.cache.size
+
+/--
+  If the element type is nullable, this returns the number of non-null elements in the cache.
+  This method requires iterating the whole array, so is slow and primarily for proofs.
+-/
+@[expose, local simp, local grind]
+def fillSlow [Nullable α] (cache : VarCache α) :=
+  cache.cache.countP Nullable.isSome
+
+@[always_inline]
+instance instGetElem : GetElem (VarCache α) Var α (fun cache var => var.idx < cache.size) where
+  getElem cache var h := cache.cache[var.idx]
+
+@[local simp, local grind =]
+private theorem getElem_eq (h : var.idx < cache.size) :
+    cache[var]'h = cache.cache[var.idx] := by
+  rfl
+
+@[always_inline]
+instance instGetElem? : GetElem? (VarCache α) Var α (fun cache var => var.idx < cache.size) where
+  getElem? cache var := cache.cache[var.idx]?
+
+instance : LawfulGetElem (VarCache α) Var α (fun cache var => var.idx < cache.size) where
+  getElem?_def := by
+    simp +instances only [instGetElem?, instGetElem]
+    grind
+
+/--
+  The membership operator is only defined for nullable caches, where a variable is a member iff
+  it references a non-null value in the cache.
+-/
+instance instMembership [Nullable α] : Membership Var (VarCache α) where
+  mem cache var := ∃ (h : var.idx < cache.size), Nullable.isSome (cache[var]'h)
+
+@[local simp, local grind =]
+theorem mem_iff [Nullable α] :
+    var ∈ cache ↔ ∃ (h : var.idx < cache.size), Nullable.isSome (cache[var]'h) := by
+  rfl
+
+@[always_inline]
+instance [Nullable α] : Decidable (var ∈ cache) := by
+  simp +instances only [instMembership]
+  infer_instance
+
+@[simp, grind =]
+theorem size_ofArray {arr : Array α} :
+    (ofArray arr).size = arr.size := by
+  grind
+
+@[simp, grind =]
+theorem getElem_ofArray {arr : Array α} (lt : var.idx < (ofArray arr).size) :
+    (ofArray arr)[var]'lt = arr[var.idx] := by
+  grind
+
+@[inline]
+def empty : VarCache α :=
+  { cache := #[] }
+
+section empty
+attribute [local simp, local grind] empty
+
+@[simp, grind =]
+theorem size_empty :
+    (empty : VarCache α).size = 0 := by
+  grind
+
+@[simp, grind =]
+theorem fillSlow_empty [Nullable α] :
+    (empty : VarCache α).fillSlow = 0 := by
+  grind
+
+@[simp, grind .]
+theorem mem_empty [Nullable α] :
+    var ∉ (empty : VarCache α) := by
+  grind
+
+end empty
+
+@[inline]
+def emptyWithCapacity (upTo : Var) : VarCache α :=
+  { cache := .emptyWithCapacity (upTo.idx + 1) }
+
+section emptyWithCapacity
+variable {upTo : Var}
+attribute [local simp, local grind] emptyWithCapacity
+
+@[simp, grind =]
+theorem size_emptyWithCapacity :
+    (emptyWithCapacity upTo : VarCache α).size = 0 := by
+  grind
+
+@[simp, grind =]
+theorem fillSlow_emptyWithCapacity [Nullable α] :
+    (emptyWithCapacity upTo : VarCache α).fillSlow = 0 := by
+  grind
+
+@[simp, grind .]
+theorem mem_emptyWithCapacity [Nullable α] :
+    var ∉ (emptyWithCapacity upTo : VarCache α) := by
+  grind
+
+end emptyWithCapacity
+
+@[inline]
+def toArray (cache : VarCache α) : Array α :=
+  cache.cache
+
+section toArray
+attribute [local simp, local grind] toArray
+
+@[simp, grind =]
+theorem size_toArray :
+    cache.toArray.size = cache.size := by
+  grind
+
+@[simp, grind =]
+theorem getElem_toArray (h : var.idx < cache.toArray.size) :
+    cache.toArray[var.idx]'h = cache[var] := by
+  grind
+
+theorem fillSlow_eq [Nullable α] :
+    cache.fillSlow = cache.toArray.countP Nullable.isSome := by
+  grind
+
+end toArray
+
+@[inline]
+def push (cache : VarCache α) (value : α) : VarCache α :=
+  { cache with cache := cache.cache.push value }
+
+section push
+variable {value : α}
+attribute [local simp, local grind] push
+
+@[simp, grind =]
+theorem size_push :
+    (cache.push value).size = cache.size + 1 := by
+  grind
+
+@[simp, grind =]
+theorem fillSlow_push [null : Nullable α] :
+    (cache.push value).fillSlow = cache.fillSlow + if null.isSome value then 1 else 0 := by
+  grind [Array.countP_push]
+
+@[simp, grind =]
+theorem mem_push [null : Nullable α] :
+    var ∈ cache.push value ↔
+    var ∈ cache ∨ (null.isSome value ∧ var.idx = cache.size) := by
+  grind
+
+@[simp, grind =]
+theorem getElem_push (lt : var.idx < (cache.push value).size) :
+    (cache.push value)[var]'lt =
+    if _ : var.idx = cache.size then value else cache[var] := by
+  grind
+
+end push
+
+@[inline]
+def set (cache : VarCache α) (var : Var) (value : α) (lt : var.idx < cache.size := by grind) : VarCache α :=
+  { cache with cache := cache.cache.set var.idx value lt }
+
+section set
+variable {value : α} (lt : var.idx < cache.size)
+attribute [local simp, local grind] set
+
+@[simp, grind =]
+theorem size_set :
+    (cache.set var value lt).size = cache.size := by
+  grind
+
+@[simp, grind =]
+theorem fillSlow_set [null : Nullable α] :
+    (cache.set var value lt).fillSlow =
+    cache.fillSlow - (if var ∈ cache then 1 else 0) + (if null.isSome value then 1 else 0) := by
+  grind
+
+@[simp, grind =]
+theorem mem_set [null : Nullable α] {var' : Var} :
+    var' ∈ cache.set var value lt ↔
+    if _ : var' = var then null.isSome value else var' ∈ cache := by
+  grind
+
+@[simp, grind =]
+theorem getElem_set {var' : Var} (lt' : var'.idx < (cache.set var value mem).size) :
+    (cache.set var value lt)[var']'lt' =
+    if _ : var' = var then value else cache[var'] := by
+  grind
+
+end set
+
+@[inline]
+def modify (cache : VarCache α) (var : Var) (lt : var.idx < cache.size := by grind) (f : { val : α // cache[var] = val } -> α) : VarCache α :=
+  { cache with cache := cache.cache.modifyMem var.idx lt f }
+
+section modify
+variable {lt : var.idx < cache.size} {f : { val : α // cache[var] = val } -> α}
+attribute [local simp, local grind] modify
+
+@[simp, grind =]
+theorem size_modify :
+    (cache.modify var lt f).size = cache.size := by
+  grind
+
+@[simp, grind =]
+theorem fillSlow_modify [null : Nullable α] :
+    (cache.modify var lt f).fillSlow =
+    cache.fillSlow - (if var ∈ cache then 1 else 0) + (if null.isSome (f ⟨cache[var], by grind⟩) then 1 else 0) := by
+  simp only [modify, fillSlow, Array.countP_modifyMem, Nullable.isSome_eq]
+  cases decide (var ∈ cache) <;> cases null.isNull (f ⟨cache[var], by grind⟩)
+  <;> grind
+
+@[simp, grind =]
+theorem mem_modify [null : Nullable α] {var' : Var} :
+    var' ∈ cache.modify var lt f ↔
+    if _ : var' = var then null.isSome (f ⟨cache[var'], by grind⟩) else var' ∈ cache := by
+  grind
+
+@[simp, grind =]
+theorem getElem_modify {var' : Var} (lt' : var'.idx < (cache.modify var lt f).size) :
+    (cache.modify var lt f)[var']'lt' =
+    if _ : var' = var then f ⟨cache[var'], by grind⟩ else cache[var'] := by
+  grind
+
+end modify
+
+def insertAbove [Nullable α] (cache : VarCache α) (var : Var) (value : α) (le : cache.size ≤ var.idx := by grind) : VarCache α :=
+  if _ : cache.size = var.idx then
+    cache.push value
+  else
+    cache.push Nullable.null |>.insertAbove var value
+termination_by var.idx - cache.size
+decreasing_by grind
+
+section insertAbove
+variable [Nullable α] {value : α} (le : cache.size ≤ var.idx)
+attribute [local grind] insertAbove
+
+@[simp, grind =]
+theorem size_insertAbove :
+    (cache.insertAbove var value le).size = var.idx + 1 := by
+  fun_induction insertAbove <;> grind
+
+@[simp, grind =]
+theorem fillSlow_insertAbove :
+    (cache.insertAbove var value le).fillSlow =
+    cache.fillSlow + if Nullable.isSome value then 1 else 0 := by
+  fun_induction insertAbove <;> grind
+
+@[simp, grind =]
+theorem mem_insertAbove {var' : Var} :
+    var' ∈ cache.insertAbove var value le ↔
+    var' ∈ cache ∨ (var' = var ∧ Nullable.isSome value) := by
+  fun_induction insertAbove <;> grind
+
+@[simp, grind =]
+theorem getElem_insertAbove {var' : Var} (lt : var'.idx < (cache.insertAbove var value le).size) :
+    (cache.insertAbove var value le)[var']'lt =
+    if var' = var then
+      value
+    else if h : var'.idx < cache.size then
+      cache[var']'h
+    else
+      Nullable.null := by
+  fun_induction insertAbove <;> grind
+
+end insertAbove
+
+@[inline]
+def insert [Nullable α] (cache : VarCache α) (var : Var) (value : α) : VarCache α :=
+  if _ : var.idx < cache.size then
+    cache.set var value
+  else
+    cache.insertAbove var value
+
+section insert
+variable [Nullable α] {value : α}
+attribute [local grind] insert
+
+@[simp, grind =]
+theorem size_insert :
+    (cache.insert var value).size = max cache.size (var.idx + 1) := by
+  grind
+
+@[simp, grind =]
+theorem fillSlow_insert :
+    (cache.insert var value).fillSlow =
+    cache.fillSlow - (if var ∈ cache then 1 else 0) + (if Nullable.isSome value then 1 else 0) := by
+  grind
+
+@[simp, grind =]
+theorem mem_insert {var' : Var} :
+    var' ∈ cache.insert var value ↔
+    if _ : var' = var then Nullable.isSome value else var' ∈ cache := by
+  grind
+
+@[simp, grind =]
+theorem getElem_insert {var' : Var} (lt : var'.idx < (cache.insert var value).size) :
+    (cache.insert var value)[var']'lt =
+    if var' = var then
+      value
+    else if h : var'.idx < cache.size then
+      cache[var']'h
+    else
+      Nullable.null := by
+  grind
+
+end insert
+
+end VarCache
+end Valaig.Data
